Modify the code structure in the index examples

fiat2/src/fiat2/PipelineEx.v
@@ -19,16 +19,19 @@ Section WithConcreteMaps.
   Instance clocals : map.map string value := SortedListString.map _.
   Instance clocals_ok : map.ok clocals := SortedListString.ok _.
 
-  Section Example1.
-    Definition sum_agg_attr := "salary".
+  Section CommonPipelineParts.
+    Context (sum_agg_attr : string).
 
-    Notation sum_agg_wf := (SumAgg.idx_wf "hole" sum_agg_attr "x").
+    Notation sum_agg_wf := (SumAgg.idx_wf (locals:=clocals) "hole" sum_agg_attr "x").
     Instance csum_agg : IndexInterface2.index := (sum_agg "hole" sum_agg_attr "x").
     Instance csum_agg_ok : IndexInterface2.ok csum_agg sum_agg_wf.
     apply sum_agg_ok.
     Qed.
 
-    Definition dict_idx_attr := "department".
+    Definition sum_agg_lookup_transf := fun tbl => fold_command_with_globals [tbl] (sum_to_agg_lookup_head sum_agg_attr "id_tag" "aux_tag" "sum_agg_tag" tbl).
+    Definition cons_to_add_transf := fun tbl => fold_command_with_globals [tbl] (cons_to_add_head).
+
+    Context (dict_idx_attr : string).
 
     Notation dict_idx_wf := (DictIndexImpl2.idx_wf "hole" dict_idx_attr "tup" "acc" "x").
     Instance cdict_idx : IndexInterface2.index := (dict_idx "hole" dict_idx_attr "tup" "acc" "x").
@@ -36,29 +39,24 @@ Section WithConcreteMaps.
     apply dict_idx_ok. auto with transf_hints.
     Qed.
 
+    Definition dict_lookup_transf := fun tbl => fold_command_with_globals [tbl] (eq_filter_to_lookup_head dict_idx_attr "id_tag" "aux_tag" "dict_idx_tag" "b" tbl).
+    Definition cons_to_insert_transf := fun tbl => fold_command_with_globals [tbl] (cons_to_insert_head dict_idx_attr "tup" "acc" "x" "y").
+    Definition use_dict_idx_transf := fun tbl => fold_command_with_globals [tbl] (use_idx_head dict_idx_attr "id_tag" "aux_tag" "dict_idx_tag" tbl).
+
     Notation pk_idx_wf := (BitmapIndex.pk_idx_wf "hole" "tup" "acc").
     Instance cpk_idx : IndexInterface2.index := (pk_idx "hole" "tup" "acc").
     Instance cpk_idx_ok : IndexInterface2.ok cpk_idx pk_idx_wf.
     apply pk_idx_ok. auto with transf_hints.
     Qed.
 
-    Definition bitmap_attr := "location".
-    Definition bitmap_str := "A".
+    Context (bitmap_attr : string).
+    Context (bitmap_str : string).
     Notation bitmap_wf := (bitmap_wf bitmap_attr bitmap_str "hole" "tup").
     Instance bitmap : IndexInterface2.index := (bitmap bitmap_attr bitmap_str "hole" "tup").
     Instance bitmap_ok : IndexInterface2.ok bitmap bitmap_wf.
     apply bitmap_ok.
     Qed.
 
-    Definition to_proj_transf := fold_command id to_proj_head.
-    Definition to_filter_transf := fold_command id to_filter_head.
-    Definition annotate_collection_transf := fold_command id annotate_collection.
-    Definition push_down_collection_transf := fold_command id push_down_collection.
-    Definition sum_agg_lookup_transf := fun tbl => fold_command_with_globals [tbl] (sum_to_agg_lookup_head sum_agg_attr "id_tag" "aux_tag" "sum_agg_tag" tbl).
-    Definition cons_to_add_transf := fun tbl => fold_command_with_globals [tbl] (cons_to_add_head).
-    Definition dict_lookup_transf := fun tbl => fold_command_with_globals [tbl] (eq_filter_to_lookup_head dict_idx_attr "id_tag" "aux_tag" "dict_idx_tag" "b" tbl).
-    Definition cons_to_insert_transf := fun tbl => fold_command_with_globals [tbl] (cons_to_insert_head dict_idx_attr "tup" "acc" "x" "y").
-    Definition use_dict_idx_transf := fun tbl => fold_command_with_globals [tbl] (use_idx_head dict_idx_attr "id_tag" "aux_tag" "dict_idx_tag" tbl).
     Definition cons_to_pk_idx_update_transf := fun tbl => fold_command_with_globals [tbl] (cons_to_pk_idx_update_head "y").
     Definition use_pk_idx_transf := fun tbl => fold_command_with_globals [tbl] (use_pk_idx_head "id_tag" "aux_tag" "pk_idx_tag" tbl).
     Definition cons_to_bitmap_update_transf := fun tbl => fold_command_with_globals [tbl] cons_to_bitmap_update_head.
@@ -66,6 +64,13 @@ Section WithConcreteMaps.
     Definition filter_to_bitmap_lookup_transf :=
       fun tbl => fold_command_with_globals [tbl]
                    (filter_to_bitmap_lookup_head bitmap_attr bitmap_str "id_tag" "aux_tag" "pk_idx_tag" "bm_tag" "x" "b" "acc" tbl).
+
+    Definition to_proj_transf := fold_command id to_proj_head.
+    Definition to_filter_transf := fold_command id to_filter_head.
+    Definition annotate_collection_transf := fold_command id annotate_collection.
+    Definition push_down_collection_transf := fold_command id push_down_collection.
+
+
 
     Notation idxs := [("sum_agg_tag", csum_agg, sum_agg_wf);
                       ("dict_idx_tag", cdict_idx, dict_idx_wf);
@@ -77,7 +82,7 @@ Section WithConcreteMaps.
     all: cbn; rewrite <- eqb_eq; intuition idtac; discriminate.
     Qed.
 
-    Definition ex_transf1 (Gstore Genv : ctenv) :=
+    Definition ex_transf (Gstore Genv : ctenv) :=
       Basics.compose
         (apply_idx_related_transfs (idx:=ccompo_idx) "id_tag" "aux_tag"
            (fun tbl =>
@@ -97,10 +102,19 @@ Section WithConcreteMaps.
               (Basics.compose annotate_collection_transf
                  (Basics.compose to_filter_transf to_proj_transf)))).
 
-    Lemma ex_transf1_sound : transf_sound (locals:=clocals) ex_transf1.
+    Lemma ex_transf_sound : transf_sound (locals:=clocals) ex_transf.
     Proof.
       repeat (repeat apply_transf_sound_lemmas; eauto 10 with transf_hints).
     Qed.
+  End CommonPipelineParts.
+
+  Section Example1.
+    Definition sum_agg_attr1 := "salary".
+    Definition dict_idx_attr1 := "department".
+    Definition bitmap_attr1 := "location".
+    Definition bitmap_str1 := "A".
+
+    Definition ex_transf1 := ex_transf sum_agg_attr1 dict_idx_attr1 bitmap_attr1 bitmap_str1.
 
     Definition row_ty := TRecord (record_sort [("name", TString); ("department", TString); ("feedback", TString); ("salary", TInt); ("location", TString)]).
     (* Two Arbitrary well_typed rows *)
@@ -143,71 +157,28 @@ Section WithConcreteMaps.
         locals_wf init_Genv1 env ->
         interp_command store env ex1_transformed = interp_command store env ex1.
     Proof.
-      apply transf_sound__preserve_sem; auto using ex_transf1_sound with transf_hints.
+      apply transf_sound__preserve_sem; eauto using ex_transf_sound with transf_hints.
     Qed.
   End Example1.
 
   Section Example2.
     Definition sum_agg_attr2 := "price".
-
-    Notation sum_agg_wf2 := (SumAgg.idx_wf "hole" sum_agg_attr2 "x").
-    Instance csum_agg2 : IndexInterface2.index := (sum_agg "hole" sum_agg_attr2 "x").
-    Instance csum_agg_ok2 : IndexInterface2.ok csum_agg2 sum_agg_wf2.
-    apply sum_agg_ok.
-    Qed.
-
     Definition dict_idx_attr2 := "color".
+    Definition bitmap_attr2 := "name".
+    Definition bitmap_str2 := "shirt_1".
 
-    Notation dict_idx_wf2 := (DictIndexImpl2.idx_wf "hole" dict_idx_attr2 "tup" "acc" "x").
-    Instance cdict_idx2 : IndexInterface2.index := (dict_idx "hole" dict_idx_attr2 "tup" "acc" "x").
-    Instance cdict_idx_ok2 : IndexInterface2.ok cdict_idx2 dict_idx_wf2.
-    apply dict_idx_ok. auto with transf_hints.
-    Qed.
-
-    Definition sum_agg_lookup_transf2 := fun tbl => fold_command_with_globals [tbl] (sum_to_agg_lookup_head sum_agg_attr2 "id_tag" "aux_tag" "sum_agg_tag" tbl).
-    Definition cons_to_add_transf2 := fun tbl => fold_command_with_globals [tbl] (cons_to_add_head).
-    Definition dict_lookup_transf2 := fun tbl => fold_command_with_globals [tbl] (eq_filter_to_lookup_head dict_idx_attr2 "id_tag" "aux_tag" "dict_idx_tag" "b" tbl).
-    Definition cons_to_insert_transf2 := fun tbl => fold_command_with_globals [tbl] (cons_to_insert_head dict_idx_attr2 "tup" "acc" "x" "y").
-    Definition use_dict_idx_transf2 := fun tbl => fold_command_with_globals [tbl] (use_idx_head dict_idx_attr2 "id_tag" "aux_tag" "dict_idx_tag" tbl).
-
-    Notation idxs2 := [("sum_agg_tag", csum_agg2, sum_agg_wf2);
-                       ("dict_idx_tag", cdict_idx2, dict_idx_wf2)].
-    Instance ccompo_idx2 : IndexInterface2.index := compo_idx idxs2 "hole" (word:=word).
-    Instance ccompo_idx_ok2 : IndexInterface2.ok ccompo_idx2 (compo_idx_wf idxs2).
-    apply compo_idx_ok; repeat constructor; intros; auto with transf_hints.
-    all: cbn; rewrite <- eqb_eq; intuition idtac; discriminate.
-    Qed.
-
-    Definition ex_transf2 (Gstore Genv : ctenv) :=
-      Basics.compose
-        (apply_idx_related_transfs (idx:=ccompo_idx2) "id_tag" "aux_tag"
-           (fun tbl =>
-              (Basics.compose (dict_lookup_transf2 tbl)
-                 (Basics.compose (use_dict_idx_transf2 tbl)
-                    (Basics.compose (repeat_transf (cons_to_insert_transf2 tbl) 10000)
-                       (Basics.compose (sum_agg_lookup_transf2 tbl)
-                          (Basics.compose (repeat_transf (cons_to_add_transf2 tbl) 10000)
-                             (cons_to_add_transf2 tbl))))))) Gstore Genv)
-        (Basics.compose push_down_collection_transf
-           (Basics.compose push_down_collection_transf
-              (Basics.compose annotate_collection_transf
-                 (Basics.compose to_filter_transf to_proj_transf)))).
-
-    Lemma ex_transf2_sound : transf_sound (locals:=clocals) ex_transf2.
-    Proof.
-      repeat (repeat apply_transf_sound_lemmas; eauto 10 with transf_hints).
-    Qed.
+    Definition ex_transf2 := ex_transf sum_agg_attr2 dict_idx_attr2 bitmap_attr2 bitmap_str2.
 
     Definition outfits_row_ty := TRecord (record_sort [("outfit_name", TString); ("shirt_name", TString); ("shirt_color", TString); ("shirt_price", TInt); ("pants_name", TString); ("pants_color", TString); ("pants_price", TInt)]).
 
     Definition shirts_row_ty := TRecord (record_sort [("name", TString); ("color", TString); ("price", TInt)]).
 
     Definition populate_shirts_from_outfits : command :=
-      CForeach (EFlatmap LikeList (ELoc "outfits") "row"
-                  (EBinop OCons
-                     (ERecord [("name", EAccess (EVar "row") "shirt_name"); ("color", EAccess (EVar "row") "shirt_color"); ("price", EAccess (EVar "row") "shirt_price")])
-                     (EAtom (ANil (Some shirts_row_ty)))))
-        "row" (CAssign "shirts" (EBinop OCons (EVar "row") (ELoc "shirts"))).
+      <{ for "row" in <[ "row" <- mut "outfits";
+                         ret ({"name" : "row" ["shirt_name"],
+                                 "color" : "row" ["shirt_color"],
+                                   "price" : "row" ["shirt_price"]}) ]>:
+                         set "shirts" := "row" :: mut "shirts" end }>.
 
     Definition filter_shirts color : expr :=
       ESort LikeList <[ "row" <- mut "shirts" ;
@@ -217,19 +188,19 @@ Section WithConcreteMaps.
     Definition query2_1 :=
       CLetMut (EAtom (AString ""))  "all_shirt_info"
         (CForeach (filter_shirts "white") "r"
-         <{ let "n" = "r"["name"] +++ << EAtom (AString ": ") >> in
+          <{ let "n" = "r"["name"] +++ << EAtom (AString ": ") >> in
             let "p" = << EUnop OIntToString (EAccess (EVar "r") "price") >> +++ << EAtom (AString "\n") >> in
             let "line" = "n" +++ "p" in
             set "all_shirt_info" := mut "all_shirt_info" +++ "line" }>).
 
     Definition query2_2 :=
-      CLetMut (EFold (<["row" <- mut "shirts" ; ret "row"["price"]]>) (EAtom (AInt 0)) "v" "acc" (EBinop OPlus (EVar "v") (EVar "acc"))) "total_shirt_price" CSkip.
+      CAssign "total_shirt_price" (EFold (<["row" <- mut "shirts" ; ret "row"["price"]]>) (EAtom (AInt 0)) "v" "acc" (EBinop OPlus (EVar "v") (EVar "acc"))).
 
     Definition ex2 := CLetMut (EAtom (ANil (Some (shirts_row_ty)))) "shirts"
                         (CSeq populate_shirts_from_outfits
                            (CSeq query2_1 query2_2)).
 
-    Definition init_Gstore2 : ctenv := map.put map.empty "outfits" (TList outfits_row_ty).
+    Definition init_Gstore2 : ctenv := map.put (map.put map.empty "outfits" (TList outfits_row_ty)) "total_shirt_price" TInt.
     Definition init_Genv2 : ctenv := map.empty.
 
     (* Compute typecheck init_Gstore2 init_Genv2 ex2. *)
@@ -242,7 +213,7 @@ Section WithConcreteMaps.
         locals_wf init_Genv2 env ->
         interp_command store env ex2_transformed = interp_command store env ex2.
     Proof.
-      apply transf_sound__preserve_sem; auto using ex_transf2_sound with transf_hints.
+      apply transf_sound__preserve_sem; eauto using ex_transf_sound with transf_hints.
     Qed.
   End Example2.
 End WithConcreteMaps.
